instead of requiring that the Cava device remembers the latest request,
pass the current request on the device's input wires

investigations/bedrock2/RiscvMachineWithCavaDevice/DetIncrMachine.v
@@ -6,95 +6,95 @@ Require Import Cava.CavaProperties.
 Section WithCava.
   Context {signal} {semantics : Cava signal}.
 
+  (* TODO doesn't Cava already provide these? *)
   Definition ite{T: SignalType}(cond: signal Bit)(thn els: signal T):
     cava (signal T) :=
     branches <- packV (Vector.of_list [els; thn]);;
     ctrl <- packV (Vector.of_list [cond]);;
     indexAt branches ctrl.
 
-  (* we need to add the Void because * is left-associative *)
-  Definition void_and_state: Type :=
-    (signal Void * signal Bit * signal Bit * signal Bit * signal Bit * signal Bit *
-     signal (Vec Bit 32) * signal (Vec Bit 32) * signal Bit).
+  Definition and3: signal Bit * signal Bit * signal Bit -> cava (signal Bit) :=
+    fun '(x1, x2, x3) => x12 <- and2 (x1, x2);; and2 (x12, x3).
 
-  (* no input/output, everything is state *)
-  Definition incr_update: void_and_state -> cava (void_and_state) :=
-    fun '(dummy_tt, pending_inp, outp_switch, idle, busy, done, value, output, output_en) =>
-      pending_inp' <- constant false;;
-      no_pending_inp <- inv pending_inp;;
-      idle' <- and2 (idle, no_pending_inp);;
-      busy' <- pending_inp;;
-      done' <- or2 (busy, done);;
-      value_plus_one <- incrN value;;
-      value' <- ite busy value_plus_one value;;
-      zeros <- Vec.const (constant false) 29;;
-      v1 <- Vec.cons done zeros;;
-      v2 <- Vec.cons busy v1;;
-      v3 <- Vec.cons idle v2;;
-      output_en' <- constant true;;
-      output' <- ite outp_switch value v3;;
-      ret (dummy_tt, pending_inp', outp_switch, idle', busy', done', value', output', output_en').
+  Definition or3: signal Bit * signal Bit * signal Bit -> cava (signal Bit) :=
+    fun '(x1, x2, x3) => x12 <- or2 (x1, x2);; or2 (x12, x3).
 
-  Definition incr: Circuit (signal Void) (signal Void) :=
-    Loop (Loop (Loop (Loop (Loop (Loop (Loop (Loop (Comb incr_update)))))))).
+  Definition incr_update:
+    (* input: *)
+    signal Bit *             (* is_read_req *)
+    signal Bit *             (* is_write_req *)
+    signal (Vec Bit 32) *    (* req_addr (only relevant if is_reaq_req or is_write_req) *)
+    signal (Vec Bit 32) *    (* req_value (only relevant if is_write_req *)
+    (* state: *)
+    signal Bit *             (* idle *)
+    signal Bit *             (* busy *)
+    signal Bit *             (* done *)
+    signal (Vec Bit 32)      (* value *)
+    -> cava (
+    (* output: *)
+    signal Bit *             (* is_resp *)
+    signal (Vec Bit 32) *    (* resp (only relevant if is_resp *)
+    (* state: *)
+    signal Bit *             (* idle *)
+    signal Bit *             (* busy *)
+    signal Bit *             (* done *)
+    signal (Vec Bit 32))     (* value *)
+  := fun '(is_read_req, is_write_req, req_addr, req_value, idle, busy, done, value) =>
+       initialized <- or3 (idle, busy, done);;
+       idle <- ite initialized idle (constant true);;
+       is_resp <- or2 (is_read_req, is_write_req);;
+       (* bit #2 of the address determines if STATUS or VALUE register *)
+       req_addr1 <- Vec.tl req_addr;;
+       req_addr2 <- Vec.tl req_addr1;;
+       is_status_req <- Vec.hd req_addr2;;
+       is_value_req <- inv is_status_req;;
+       is_value_write_req <- and2 (is_value_req, is_write_req);;
+       no_pending_inp <- inv is_resp;;
+       idle' <- and2 (idle, no_pending_inp);;
+       busy' <- is_value_write_req;;
+       done' <- or2 (busy, done);;
+       value_plus_one <- incrN value;;
+       value_or_input <- ite is_value_write_req req_value value;;
+       value' <- ite busy value_plus_one value_or_input;;
+       zeros <- Vec.const (constant false) 29;;
+       v1 <- Vec.cons done zeros;;
+       v2 <- Vec.cons busy v1;;
+       v3 <- Vec.cons idle v2;;
+       resp <- ite is_status_req v3 value;;
+       ret (is_resp, resp, idle', busy', done', value').
+
+  Definition incr: Circuit (signal Bit * signal Bit * signal (Vec Bit 32) * signal (Vec Bit 32))
+                           (signal Bit * signal (Vec Bit 32)) :=
+    Loop (Loop (Loop (Loop (Comb incr_update)))).
 
 End WithCava.
 
-Definition device_state: Type := Eval simpl in circuit_state incr.
-
-Definition get_output: device_state -> Vector.t bool 32 :=
-  fun '(_, (_, (_, (_, (_, (_, (_, (_, (_, output_en), output),
-                                value), done), busy), idle), outp_switch), pending_inp)) => output.
-
-Definition get_output_en: device_state -> bool :=
-  fun '(_, (_, (_, (_, (_, (_, (_, (_, (_, output_en), output),
-                                value), done), busy), idle), outp_switch), pending_inp)) => output_en.
-
-Definition get_pending_inp: device_state -> bool :=
-  fun '(_, (_, (_, (_, (_, (_, (_, (_, (_, output_en), output),
-                                value), done), busy), idle), outp_switch), pending_inp)) => pending_inp.
-
-Definition set_outp_switch(b: bool): device_state -> device_state :=
-  fun '(_, (_, (_, (_, (_, (_, (_, (_, (_, output_en), output),
-                                value), done), busy), idle), outp_switch), pending_inp)) =>
-    (tt, (tt, (tt, (tt, (tt, (tt, (tt, (tt, (tt, output_en), output),
-                                   value), done), busy), idle), b), pending_inp)).
-
-Definition set_outp_en(b: bool): device_state -> device_state :=
-  fun '(_, (_, (_, (_, (_, (_, (_, (_, (_, output_en), output),
-                                value), done), busy), idle), outp_switch), pending_inp)) =>
-    (tt, (tt, (tt, (tt, (tt, (tt, (tt, (tt, (tt, b), output),
-                                   value), done), busy), idle), outp_switch), pending_inp)).
-
-Definition set_pending_inp(b: bool): device_state -> device_state :=
-  fun '(_, (_, (_, (_, (_, (_, (_, (_, (_, output_en), output),
-                                value), done), busy), idle), outp_switch), pending_inp)) =>
-    (tt, (tt, (tt, (tt, (tt, (tt, (tt, (tt, (tt, output_en), output),
-                                   value), done), busy), idle), outp_switch), b)).
-
-Definition set_value(v: Vector.t bool 32): device_state -> device_state :=
-  fun '(_, (_, (_, (_, (_, (_, (_, (_, (_, output_en), output),
-                                value), done), busy), idle), outp_switch), pending_inp)) =>
-    (tt, (tt, (tt, (tt, (tt, (tt, (tt, (tt, (tt, output_en), output),
-                                   v), done), busy), idle), outp_switch), pending_inp)).
-
-Definition incr_device_step(state: device_state): device_state :=
-  fst (step incr state tt).
+Definition incr_device_step:
+  (* input: current state, is_read_req, is_write_req, req_addr, req_value *)
+  circuit_state incr -> bool * bool * Bvector 32 * Bvector 32 ->
+  (* output: next state, is_resp, resp *)
+  circuit_state incr * (bool * Bvector 32)
+  := step incr.
 
 Require Import coqutil.Datatypes.List.
 
-Example sample_trace := Eval compute in
-  let done := false in
-  let busy := false in
-  let idle := true in
-  let outp_switch := false in
-  let pending_inp := true in
-  let output := Vector.const false 32 in
-  let output_en := false in
-  let value := (Vector.const true 2 ++ Vector.const false 30)%vector in
-  let start := (tt, (tt, (tt, (tt, (tt, (tt, (tt, (tt, (tt,
-      output_en), output), value), done), busy), idle), outp_switch), pending_inp)) in
-  List.unfoldn incr_device_step 5 start.
+(* like `simulate`, but also output the internal state, for more insightful debugging *)
+Fixpoint simulate_with_state_rec{i o}(c: Circuit i o)(initial: circuit_state c)(inps: list i)
+  : list (circuit_state c * o) :=
+  match inps with
+  | [] => []
+  | inp :: rest => let r := step c initial inp in r :: simulate_with_state_rec c (fst r) rest
+  end.
+Definition simulate_with_state{i o}(c: Circuit i o): list i -> list (circuit_state c * o) :=
+  simulate_with_state_rec c (reset_state c).
+
+Example sample_trace := Eval compute in simulate_with_state incr [
+  (false, false, N2Bv_sized 32 111, N2Bv_sized 32 111); (* no action *)
+  (false, true, N2Bv_sized 32 0, N2Bv_sized 32 15);     (* write VALUE:=15 *)
+  (true, false, N2Bv_sized 32 4, N2Bv_sized 32 111);    (* read STATUS *)
+  (true, false, N2Bv_sized 32 4, N2Bv_sized 32 111);    (* read STATUS *)
+  (true, false, N2Bv_sized 32 0, N2Bv_sized 32 111)     (* read VALUE *)
+].
 
 (* Print sample_trace. *)
 
@@ -109,40 +109,12 @@ Section WithParameters.
   Context {word: Interface.word 32} {word_ok: word.ok word}
           {Mem: map.map word byte} {Registers: map.map Z word}.
 
-  Definition bv_to_word(v: Vector.t bool 32): word :=
-    word.of_Z (Z.of_N (Bv2N v)).
-
-  Definition word_to_bv(w: word): Vector.t bool 32 :=
-    N2Bv_sized 32 (Z.to_N (word.unsigned w)).
-
   Global Instance counter_device: device := {|
-    device.state := device_state;
-
-    device.reset_state :=
-      (tt, (tt, (tt, (tt, (tt, (tt, (tt, (tt, (tt, false),
-                                          word_to_bv (word.of_Z 0)), word_to_bv (word.of_Z 0)),
-                                false), false), true), false), false));
-
+    device.state := circuit_state incr;
+    device.reset_state := reset_state incr;
     device.run1 := incr_device_step;
-
-    device.addr_range_start := word.of_Z INCR_BASE_ADDR;
-    device.addr_range_pastend := word.of_Z INCR_END_ADDR;
-
-    device.readReq(num_bytes: nat)(addr: word)(s: device_state) :=
-      (* TODO the address-to-register mapping could/should also be implemented in Cava *)
-      set_outp_en false (set_outp_switch (word.eqb (word.of_Z 0) (word.and addr (word.of_Z 4))) s);
-      (* outp_en will be set to true as soon as one cycle is run, which can set output
-         according to outp_switch *)
-
-    device.readResp(s: device_state) :=
-      if get_output_en s then Some (bv_to_word (get_output s)) else None;
-
-    device.writeReq(num_bytes: nat)(addr value: word)(s: device_state) :=
-      set_value (word_to_bv value) (set_pending_inp true s);
-
-    device.writeResp(s: device_state) :=
-      if get_pending_inp s then None else Some tt;
-
+    device.addr_range_start := INCR_BASE_ADDR;
+    device.addr_range_pastend := INCR_END_ADDR;
     device.maxRespDelay := 1;
   |}.
 
